proof.dfy
@@ -18,22 +18,99 @@ module Proof {
   import opened SafetySpec
 
   // Here's a predicate that will be very useful in constructing inviariant conjuncts.
-  predicate InFlight(c:Constants, v:Variables, message:Host.Message) {
-    && v.WF(c)
-    && message in v.network.sentMsgs
-    && false // ...and then add a check that the message's epoch is still valid.
+  predicate CommitAgreement(c:Constants, v:Variables) {
+    && (forall msg1, msg2 | 
+        && msg1 in v.network.sentMsgs 
+        && msg2 in v.network.sentMsgs 
+        && msg1.seqID == msg2.seqID
+        && msg1.Commit?
+        && msg2.Commit?
+        :: msg1 == msg2)
   }
 
 
   predicate Inv(c: Constants, v:Variables) {
-    true // Replace this placeholder with an invariant that's inductive and supports Safety.
+    && CommitAgreement(c, v)
   }
 
-  lemma SafetyProof(c: Constants, v:Variables, v':Variables)
+  function getAllPreparesForSeqID(c: Constants, v:Variables, seqID:Host.SequenceID) : set<Host.Message> 
+  {
+    set msg | && msg in v.network.sentMsgs 
+                 && msg.Prepare?
+                 && msg.seqID == seqID 
+  }
+
+  predicate QuorumOfPreparesInNetwork(c: Constants, v:Variables, seqID:Host.SequenceID) {
+    && |getAllPreparesForSeqID()| >= Host.AgreementQuorum()
+  }
+
+  lemma WlogCommitAgreement(c: Constants, v:Variables, v':Variables, step:Step, h_step:Host.Step,
+                            old_msg:Host.Message, new_msg:Host.Message)
+    requires NextStep(c, v, v', step)
+    requires  var h_c := c.hosts[step.id];
+              var h_v := v.hosts[step.id];
+              var h_v' := v'.hosts[step.id];
+              && Host.NextStep(h_c, h_v, h_v', step.msgOps, h_step)
+              && h_step.SendCommitStep?
+              && Host.SendCommit(h_c, h_v, h_v', step.msgOps, h_step.seqID)
+              
+    requires Inv(c, v)
+    ensures old_msg == new_msg
+  {
+    assert QuorumOfPreparesInNetwork(h_c, h_v, h_step.seqID, old_msg.clientOp);
+    assert QuorumOfPreparesInNetwork(h_c, h_v, h_step.seqID, new_msg.clientOp);
+  }
+
+  lemma InvariantNext(c: Constants, v:Variables, v':Variables)
+    requires Inv(c, v)
+    requires Next(c, v, v')
+    ensures Inv(c, v')
+  {
+    var step :| NextStep(c, v, v', step);
+    var h_c := c.hosts[step.id];
+    var h_v := v.hosts[step.id];
+    var h_v' := v'.hosts[step.id];
+    var h_step :| Host.NextStep(h_c, h_v, h_v', step.msgOps, h_step);
+    match h_step
+      case SendPrePrepareStep() => { assert Inv(c, v'); }
+      case RecvPrePrepareStep => { assert Inv(c, v'); }
+      case SendPrepareStep(seqID) => { assert Inv(c, v'); }
+      case RecvPrepareStep => { assert Inv(c, v'); }
+      case SendCommitStep(seqID) => {
+        forall msg1, msg2 | 
+          && msg1 in v'.network.sentMsgs 
+          && msg2 in v'.network.sentMsgs 
+          && msg1.seqID == msg2.seqID
+          && msg1.Commit?
+          && msg2.Commit?
+          ensures msg1 == msg2 {
+            if(msg1 in v.network.sentMsgs && msg2 in v.network.sentMsgs) {
+              assert msg1 == msg2;
+            } else if(msg1 !in v.network.sentMsgs && msg2 !in v.network.sentMsgs) {
+              assert msg1 == msg2;
+            } else if(msg1 in v.network.sentMsgs && msg2 !in v.network.sentMsgs) {
+              WlogCommitAgreement(c, v, v', step, h_step, msg1, msg2);
+              assert msg1 == msg2;
+            } else if(msg1 !in v.network.sentMsgs && msg2 in v.network.sentMsgs) {
+              WlogCommitAgreement(c, v, v', step, h_step, msg2, msg1);
+              assert msg1 == msg2;
+            } else {
+              assert false;
+            }
+            
+          }
+          assert Inv(c, v'); 
+      }
+
+  }
+
+  lemma InvariantInductive(c: Constants, v:Variables, v':Variables)
     ensures Init(c, v) ==> Inv(c, v)
     ensures Inv(c, v) && Next(c, v, v') ==> Inv(c, v')
-    ensures Inv(c, v) ==> Safety(c, v)
+    //ensures Inv(c, v) ==> Safety(c, v)
   {
-    // Develop any necessary proof here.
+    if Inv(c, v) && Next(c, v, v') {
+      InvariantNext(c, v, v');
+    }
   }
 }
